theories/lang/pagetable_extra.v
@@ -1,5 +1,5 @@
 From HypVeri Require Import machine machine_extra tactics.
-From HypVeri.algebra Require Import base base_extra.
+From HypVeri.algebra Require Import base base_extra pagetable.
 
 Section pagetable_extra.
 
@@ -74,7 +74,6 @@ Proof.
   induction ps as [|p ps] using set_ind_L.
   done.
   intro.
-  (* rewrite /update_ownership /=. *)
   rewrite set_fold_disj_union_strong.
   {
     rewrite set_fold_singleton /=.
@@ -239,45 +238,306 @@ Proof.
 Qed.
 
 
+Lemma p_flip_excl_current_vm σ i (ps: gset PID) :
+ get_current_vm (update_page_table_global flip_excl σ i ps) = get_current_vm σ.
+Proof. f_equal. Qed.
 
+Lemma p_flip_excl_regs σ i (ps: gset PID):
+ get_reg_files (update_page_table_global flip_excl σ i ps) = get_reg_files σ.
+Proof. f_equal. Qed.
 
+Lemma p_flip_excl_mem σ i (ps: gset PID):
+ get_mem (update_page_table_global flip_excl σ i ps) = get_mem σ.
+Proof. f_equal. Qed.
+
+Lemma p_flip_excl_mb σ i (ps: gset PID):
+ get_mail_boxes (update_page_table_global flip_excl σ i ps) = get_mail_boxes σ.
+Proof. f_equal. Qed.
+
+Lemma p_flip_excl_trans σ i (ps: gset PID):
+ get_transactions (update_page_table_global flip_excl σ i ps) = get_transactions σ.
+Proof. f_equal. Qed.
+
+Lemma p_flip_excl_own σ i ps:
+ (get_own_gmap (update_page_table_global flip_excl σ i ps)) = (get_own_gmap σ).
+Proof.
+  rewrite /get_own_gmap /=.
+  generalize dependent σ.1.1.1.2.
+  induction ps as [|p ps] using set_ind_L.
+  done.
+  intro.
+  rewrite set_fold_disj_union_strong.
+  {
+    rewrite set_fold_singleton /=.
+  set pgt' := (X in X !! p).
+  destruct (pgt' !! p) eqn:Hlookup.
+  { destruct p1.
+    rewrite IHps /=.
+    rewrite fmap_insert /=.
+    apply map_eq.
+    intro.
+    destruct (decide (i0=p)).
+    rewrite e.
+    rewrite lookup_insert.
+    destruct p1.
+    rewrite lookup_fmap Hlookup //.
+    rewrite lookup_insert_ne;[done|eauto].
+  }
+  rewrite IHps //.
+  }
+  apply upd_is_strong_assoc_comm.
+  { set_solver + H. }
+  Qed.
+
+Lemma p_flip_excl_acc σ i ps:
+ (get_access_gmap (update_page_table_global flip_excl σ i ps)) = (get_access_gmap σ).
+Proof.
+  rewrite /get_access_gmap  /=.
+  generalize dependent σ.1.1.1.2.
+  induction ps as [|p ps] using set_ind_L.
+  done.
+  intro.
+  rewrite set_fold_disj_union_strong.
+  {
+    rewrite set_fold_singleton /=.
+  set pgt' := (X in X !! p).
+  destruct (pgt' !! p) eqn:Hlookup.
+  { destruct p1.
+    rewrite IHps /=.
+    f_equal.
+    apply (list_eq_same_length _ _ vm_count).
+    rewrite fmap_length.
+    apply length_list_of_vmids.
+    rewrite fmap_length.
+    apply length_list_of_vmids.
+    intros ? ? ? ? H0 H1.
+    apply list_lookup_fmap_inv in H0, H1.
+    destruct H0, H1.
+    destruct H0, H1.
+    rewrite H3 in H4.
+    inversion H4. subst x1.
+    clear H4.
+    rewrite H0 H1.
+    do 4 f_equal.
+    destruct p1.
+    destruct o;
+    rewrite fmap_insert insert_id //.
+    all: rewrite /= lookup_fmap Hlookup //.
+  }
+  rewrite IHps //.
+  }
+  apply upd_is_strong_assoc_comm.
+  { set_solver + H. }
+Qed.
 
 Lemma u_grnt_acc_acc σ ps v sacc:
+  set_Forall (λ p, is_Some ((get_page_table σ) !! p)) ps ->
   get_access_gmap σ !! v = Some (to_dfrac_agree (DfracOwn 1) sacc) ->
   get_access_gmap (update_page_table_global grant_access σ v ps)
   =  <[v := to_dfrac_agree (DfracOwn 1) (ps ∪ sacc)]>(get_access_gmap σ).
 Proof.
-Admitted.
-  (* rewrite /get_access_gmap. *)
-  (* rewrite /revoke_access_global /update_page_table_global /=. *)
-  (* rewrite /revoke_acc_gmap /update_acc_gmap /=. *)
-  (* generalize  σ.1.1.1.2. *)
-  (* induction ps as [|p ps] using set_ind_L. *)
-  (* intros. *)
-  (* rewrite !set_fold_empty //. *)
-  (* intro pgt. *)
-  (* rewrite !set_fold_disj_union_strong /=. *)
-  (* rewrite !set_fold_singleton. *)
-  (* rewrite IHps. *)
-  (* rewrite lookup_fmap. *)
-  (* destruct (pgt!! p) eqn:Hlookup. *)
-  (* { rewrite Hlookup /=. *)
-  (*   destruct p0. *)
-  (*   simpl. *)
-  (*   f_equal. *)
-  (*   rewrite fmap_insert //=. *)
-  (* } *)
-  (* { rewrite Hlookup //=. } *)
-  (* 2,4 : set_solver + H. *)
-  (* { *)
-  (*   intros. *)
-  (*   destruct (b' !! x2) as [p2|] eqn: Hlookup2, (b' !! x1) as [p1|] eqn:Hlookup1; *)
-  (*     try destruct p1 as [q1 []]; try destruct p2 as [q2 []]; rewrite ?lookup_insert_ne ?Hlookup1 ?Hlookup2 //;last eauto. *)
-  (*   apply insert_commute. *)
-  (*   done. *)
-  (* } *)
-  (* apply upd_is_strong_assoc_comm. *)
-(* Qed. *)
+  rewrite /grant_access /update_page_table_global /=.
+  repeat destruct σ as [σ ?].
+  simpl.
+  intros Hforall Hlk.
+  apply map_eq.
+  intro.
+  destruct (decide (i = v)).
+  { subst.
+    rewrite lookup_insert.
+    revert Hforall Hlk.
+    generalize p.
+    generalize sacc.
+    induction ps as [|p' ps] using set_ind_L.
+    intros ? ? Hlk.
+    rewrite !set_fold_empty //.
+    rewrite union_empty_l_L //.
+    intros ? ?  Hlk.
+    rewrite !set_fold_disj_union_strong /=.
+    rewrite !set_fold_singleton.
+    destruct (p0 !! p') eqn: Hlk_p'.
+    2:{
+      specialize (Hlk p'). feed specialize Hlk.
+      set_solver.
+      simpl in Hlk.
+      rewrite Hlk_p' in Hlk.
+      inversion Hlk. done.
+    }
+    intro Hlookup.
+    rewrite (IHps ({[p']} ∪ sacc0)).
+    assert (ps ∪ ({[p']} ∪ sacc0) = {[p']} ∪ ps ∪ sacc0) as ->.
+    set_solver +.
+    done.
+    rewrite /get_access_gmap.
+    destruct p1.
+    intros p2 Hin_p2.
+    destruct (decide (p2 = p')).
+    { subst p2. rewrite lookup_insert. done. }
+    { rewrite lookup_insert_ne //. apply Hlk. set_solver + Hin_p2. }
+    rewrite /get_access_gmap /=.
+    rewrite fmap_insert /=.
+    destruct p1.
+    simpl.
+    rewrite -elem_of_list_to_map.
+    2:{
+      rewrite -list_fmap_compose.
+      simpl.
+      rewrite NoDup_fmap.
+      apply NoDup_list_of_vmids.
+    }
+    apply elem_of_list_In.
+    apply in_map_iff.
+    exists v.
+    split;auto.
+    2: apply in_list_of_vmids.
+    f_equal.
+    f_equal.
+    rewrite (map_filter_insert_True _ _ p').
+    2: { set_solver. }
+    rewrite dom_insert_L.
+    f_equal.
+    rewrite /get_access_gmap in Hlookup.
+    rewrite -elem_of_list_to_map in Hlookup.
+    2:{
+      rewrite -list_fmap_compose.
+      simpl.
+      rewrite NoDup_fmap.
+      apply NoDup_list_of_vmids.
+    }
+    apply elem_of_list_In in Hlookup.
+    apply in_map_iff in Hlookup.
+    destruct Hlookup as [? [Heq _]].
+    inversion Heq.
+    done.
+    2: set_solver + H.
+    {
+      intros.
+      destruct (b' !! x2) as [p2|] eqn: Hlookup2, (b' !! x1) as [p1|] eqn:Hlookup1;
+        rewrite ?lookup_insert_ne ?Hlookup1 ?Hlookup2 //;last eauto.
+      rewrite insert_commute //.
+    }
+  }
+  { rewrite lookup_insert_ne //.
+    destruct (get_access_gmap (σ, t0, p, v0, m, t) !! i) eqn: Hlookup.
+    {
+    revert Hforall Hlookup.
+    generalize p.
+    generalize sacc.
+    induction ps as [|p' ps] using set_ind_L.
+    intros ? ? Hforall.
+    rewrite !set_fold_empty //.
+    intros ? ?  Hforall Hlookup.
+    rewrite !set_fold_disj_union_strong /=.
+    rewrite !set_fold_singleton.
+    destruct (p0 !! p') eqn: Hlk_p'.
+    2:{
+      specialize (Hforall p'). feed specialize Hforall.
+      set_solver.
+      simpl in Hforall.
+      rewrite Hlk_p' in Hforall.
+      inversion Hforall. done.
+    }
+    rewrite (IHps ({[p']} ∪ sacc0)) //.
+    destruct p1.
+    intros p2 Hin_p2.
+    destruct (decide (p2 = p')).
+    { subst p2. rewrite lookup_insert. done. }
+    { rewrite lookup_insert_ne //. apply Hforall. set_solver + Hin_p2. }
+    rewrite /get_access_gmap /=.
+    rewrite fmap_insert /=.
+    destruct p1.
+    simpl.
+    rewrite -elem_of_list_to_map.
+    2:{
+      rewrite -list_fmap_compose.
+      simpl.
+      rewrite NoDup_fmap.
+      apply NoDup_list_of_vmids.
+    }
+    apply elem_of_list_In.
+    apply in_map_iff.
+    exists i.
+    split;auto.
+    2: apply in_list_of_vmids.
+    f_equal.
+    (* rewrite (map_filter_insert _ _ p'). *)
+    (* rewrite dom_insert_L. *)
+    (* f_equal. *)
+    rewrite /get_access_gmap in Hlookup.
+    rewrite -elem_of_list_to_map in Hlookup.
+    2:{
+      rewrite -list_fmap_compose.
+      simpl.
+      rewrite NoDup_fmap.
+      apply NoDup_list_of_vmids.
+    }
+    apply elem_of_list_In in Hlookup.
+    apply in_map_iff in Hlookup.
+    destruct Hlookup as [? [Heq _]].
+    inversion Heq.
+    subst x.
+    f_equal.
+    destruct (decide (i ∈ g)).
+    rewrite (map_filter_insert_True _ _ p').
+    2: { set_solver + e. }
+    rewrite dom_insert_L.
+    assert (p' ∈ dom (gset PID) (filter (λ kv : PID * gset VMID, i ∈ kv.2) ((λ p2 : option VMID * bool * gset VMID, p2.2) <$> p0))).
+    {
+      rewrite elem_of_dom.
+      exists g.
+      rewrite map_filter_lookup_Some.
+      split;auto.
+      rewrite lookup_fmap_Some.
+      exists (p1,g).
+      split;done.
+    }
+    set_solver + H0.
+    rewrite (map_filter_insert_False _ _ p').
+    2: { set_solver + n0 n. }
+    rewrite map_filter_delete.
+    rewrite dom_delete_L.
+    assert (p' ∉ dom (gset PID) (filter (λ kv : PID * gset VMID, i ∈ kv.2) ((λ p2 : option VMID * bool * gset VMID, p2.2) <$> p0))).
+    {
+      rewrite elem_of_dom.
+      intro.
+      destruct H0.
+      rewrite map_filter_lookup_Some in H0.
+      destruct H0.
+      rewrite lookup_fmap_Some in H0.
+      destruct H0.
+      destruct H0.
+      subst x.
+      rewrite H3 in Hlk_p'.
+      inversion Hlk_p'.
+      subst x0.
+      set_solver + H1 n0.
+    }
+    set_solver + H0.
+    2: set_solver + H.
+    {
+      intros.
+      destruct (b' !! x2) as [p2|] eqn: Hlookup2, (b' !! x1) as [p1|] eqn:Hlookup1;
+        rewrite ?lookup_insert_ne ?Hlookup1 ?Hlookup2 //;last eauto.
+      rewrite insert_commute //.
+    }
+    }
+    rewrite /get_access_gmap in Hlookup.
+    rewrite -not_elem_of_list_to_map in Hlookup.
+    exfalso.
+    apply Hlookup.
+    rewrite -list_fmap_compose.
+    rewrite /fst.
+    cbn.
+    set F := ((λ p0 : VMID * dfrac_agreeR (gsetO PID), let (x, _) := p0 in x)
+                ∘ (λ i0 : fin vm_count,
+                      (i0, to_frac_agree 1 (dom (gset PID) (filter (λ kv : PID * gset VMID, i0 ∈ kv.2) ((λ p0 : option VMID * bool * gset VMID, p0.2) <$> p)))))).
+    apply <- (elem_of_list_fmap (A:= fin vm_count) (B:= VMID)).
+    exists i.
+    split. done.
+    rewrite elem_of_list_In.
+    apply in_list_of_vmids.
+  }
+Qed.
 
 
 
