theories/rules/mem_send.v
@@ -8,6 +8,26 @@ Section mem_send.
 Context `{hypparams: HypervisorParameters}.
 Context `{vmG: !gen_VMG Σ}.
 
+Lemma parse_transaction_descriptor_tx mem_tx mem p_tx len tran:
+ parse_transaction_descriptor mem_tx (of_pid p_tx) len = Some tran ->
+ map_Forall (λ k v, mem !! k = Some v) mem_tx ->
+ parse_transaction_descriptor mem (of_pid p_tx) len = Some tran.
+Proof.
+  rewrite /parse_transaction_descriptor.
+  rewrite /parse_list_of_Word.
+  intros Hparse Hforall.
+  destruct (sequence_a (map (λ v : Addr, mem_tx !! v) (finz.seq p_tx len))) eqn:Heqn;last done.
+  assert (sequence_a (map (λ v : Addr, mem !! v) (finz.seq p_tx len)) = Some l) as ->.
+  {
+    apply (sequence_a_map_subseteq _ _ _ mem_tx). done.
+    rewrite map_subseteq_spec.
+    intros.
+    apply Hforall.
+    done.
+  }
+  done.
+Qed.
+
 Lemma mem_send_invalid_len {i wi r0 r1 r2 hvcf tt q sacc p_tx} ai :
   (tpa ai) ∈ sacc ->
   (tpa ai) ≠ p_tx ->
@@ -322,6 +342,100 @@ Lemma mem_share {i wi r0 r1 r2 hvcf p_tx sacc} ai j mem_tx sh (ps: gset PID) :
                  TX@ i := p_tx ∗
                  memory_page p_tx mem_tx}}}.
 Proof.
+  iIntros (Hin_acc Hneq_tx len Hdecode_i Hdecode_f Htt Hle_ps Hparse Hneq_vmid Hsubseteq_acc Hneq_hp Φ)
+          "(>PC & >mem_ins & >oe & >acc & >R0 & >R1 & >R2 & >[hp handles] & >tx & >mem_tx) HΦ".
+  iApply (sswp_lift_atomic_step ExecI);[done|].
+  iIntros (n σ1) "%Hsche state".
+  rewrite /scheduled /= /scheduler in Hsche.
+  assert (σ1.1.1.2 = i) as Heq_cur. { case_bool_decide;last done. by apply fin_to_nat_inj. }
+  clear Hsche.
+  iModIntro.
+  iDestruct "state" as "(Hnum & mem & regs & mb & rx_state & pgt_owned & pgt_acc & pgt_excl &
+                            trans & hpool & retri & %Hwf & %Hconsis & %Hdisj)".
+  (* valid regs *)
+  iDestruct ((gen_reg_valid4 i PC ai R0 r0 R1 r1 R2 r2 Heq_cur) with "regs PC R0 R1 R2")
+    as "(%Hlookup_PC & %Hlookup_R0 & %Hlookup_R1 & %Hlookup_R2)";eauto.
+  (* valid pt *)
+  iDestruct (access_agree_check_true (tpa ai) i with "pgt_acc acc") as %Hcheckpg_ai;eauto.
+  iDestruct (access_agree_check_true_forall with "pgt_acc acc") as %Hcheckpg_acc;eauto.
+  iDestruct (big_sepS_sep with "oe") as "[own excl]".
+  iDestruct (excl_agree_Some_check_true_bigS with "pgt_excl excl") as %Hcheckpg_excl;eauto.
+  iDestruct (own_agree_Some_check_true_bigS with "pgt_owned own") as %Hcheckpg_own;eauto.
+  (* valid mem *)
+  iDestruct (gen_mem_valid ai wi with "mem mem_ins") as %Hlookup_ai.
+  iDestruct (gen_mem_valid_SepM with "mem [mem_tx]") as %Hlookup_mem_tx.
+  { iDestruct "mem_tx" as "[% mem_tx]". iExact "mem_tx". }
+  (* valid tx *)
+  iDestruct (mb_valid_tx i p_tx with "mb tx") as %Heq_tx.
+  (* valid hpool *)
+  iDestruct (hpool_valid with "hpool hp") as %Heq_hp.
+  iSplit.
+  - (* reducible *)
+    iPureIntro.
+    apply (reducible_normal i Hvc ai wi);eauto.
+    rewrite Heq_tx //.
+  - iModIntro.
+    iIntros (m2 σ2) "vmprop_auth %HstepP".
+    iFrame "vmprop_auth".
+    apply (step_ExecI_normal i Hvc ai wi) in HstepP;eauto.
+    2: rewrite Heq_tx //.
+    remember (exec Hvc σ1) as c2 eqn:Heqc2.
+    destruct hvcf; inversion Htt.
+    rewrite /exec /hvc Hlookup_R0 /= Hdecode_f /mem_send Hlookup_R1 /= in Heqc2.
+    case_bool_decide;first lia.
+    rewrite -Heq_tx -Heq_cur /len in Hparse.
+    apply (parse_transaction_descriptor_tx _ σ1.1.2) in Hparse;last done.
+    rewrite Hparse //= in Heqc2.
+    case_bool_decide.
+    2: { destruct H1. split;auto. split;eauto. rewrite Heq_cur //. }
+    case_bool_decide.
+    2: { destruct H2. intros s Hin.
+         rewrite Heq_cur.
+         rewrite andb_true_iff. split.
+         rewrite /check_excl_access_page.
+         rewrite andb_true_iff. split.
+         apply Hcheckpg_acc.
+         set_solver + Hsubseteq_acc Hin.
+         by apply Hcheckpg_excl.
+         by apply Hcheckpg_own.
+    }
+    rewrite /new_transaction /= /fresh_handle /= -Heq_hp in Heqc2.
+    destruct (elements sh) as [| h fhs] eqn:Hfhs.
+    { exfalso. rewrite -elements_empty in Hfhs.  apply Hneq_hp. apply set_eq.
+      intro. rewrite -elem_of_elements Hfhs elem_of_elements. split;intro;set_solver. }
+    destruct HstepP;subst m2 σ2; subst c2; simpl.
+    rewrite /gen_vm_interp.
+    (* unchanged part *)
+    rewrite (preserve_get_mb_gmap σ1).
+    rewrite (preserve_get_rx_gmap σ1).
+    all: try rewrite p_upd_pc_mb //.
+    rewrite p_upd_pc_mem 2!p_upd_reg_mem p_flip_excl_mem p_alloc_trans_mem.
+    iFrame "Hnum mem rx_state mb".
+    (* upd regs *)
+    rewrite Heq_cur.
+    rewrite (u_upd_pc_regs _ i ai) //.
+    2: { rewrite 2!u_upd_reg_regs.
+         rewrite (preserve_get_reg_gmap σ1). rewrite lookup_insert_ne //.  rewrite lookup_insert_ne //. solve_reg_lookup. done.
+    }
+    rewrite u_upd_reg_regs p_upd_reg_current_vm p_flip_excl_current_vm p_alloc_trans_current_vm  Heq_cur.
+    rewrite u_upd_reg_regs p_flip_excl_current_vm p_alloc_trans_current_vm  Heq_cur.
+    rewrite (preserve_get_reg_gmap σ1) //.
+    iDestruct ((gen_reg_update3_global PC i (ai ^+ 1)%f R2 i h R0 i (encode_hvc_ret_code Succ)) with "regs PC R2 R0")
+      as ">[$ [PC [R2 R0]]]";eauto.
+    (* upd pgt *)
+    rewrite (preserve_get_own_gmap (update_page_table_global flip_excl (alloc_transaction σ1 h (i, j, ps, Sharing, false)) i ps) (update_incr_PC _)).
+    2: rewrite p_upd_pc_pgt !p_upd_reg_pgt //.
+    rewrite p_flip_excl_own. rewrite (preserve_get_own_gmap σ1) //.
+    iFrame "pgt_owned".
+    rewrite (preserve_get_access_gmap (update_page_table_global flip_excl (alloc_transaction σ1 h (i, j, ps, Sharing, false)) i ps) (update_incr_PC _)).
+    2: rewrite p_upd_pc_pgt p_upd_reg_pgt //.
+    rewrite p_flip_excl_acc. rewrite (preserve_get_access_gmap σ1) //.
+    iFrame "pgt_acc".
+    rewrite (preserve_get_excl_gmap (update_page_table_global flip_excl (alloc_transaction σ1 h (i, j, ps, Sharing, false)) i ps) (update_incr_PC _)).
+    2: rewrite p_upd_pc_pgt p_upd_reg_pgt //.
+
+    (* rewrite (preserve_get_excl_gmap σ1) //. *)
+    (* iFrame "pgt_excl". *)
 Admitted.
 
 Lemma mem_lend {i wi r0 r1 r2 hvcf p_tx sacc} ai j mem_tx sh (ps: gset PID) :
